update SLL prediction module

parser/SLLPrediction.v
@@ -12,9 +12,7 @@ Module SllPredictionFn (Import D : Defs.T).
 
   (* move operation *)
 
-  Definition sll_moveSp (t : token) (sp : sll_subparser) : subparser_move_result :=
-    match t with
-    | @existT _ _ a _ =>
+  Definition sllMoveSp (a : terminal) (sp : sll_subparser) : subparser_move_result :=
       match sp with
       | SllSp pred stk =>
         match stk with
@@ -27,25 +25,108 @@ Module SllPredictionFn (Import D : Defs.T).
           else
             MoveReject
         end
-      end
-    end.
+      end.
 
-  Definition sll_move (t : token) (sps : list sll_subparser) : move_result sll_subparser :=
-    aggrMoveResults (map (sll_moveSp t) sps).
+  Lemma sllMoveSp_preserves_prediction :
+    forall t sp sp',
+      sllMoveSp t sp = MoveSucc sp'
+      -> sp'.(sll_prediction) = sp.(sll_prediction).
+  Proof.
+    intros t sp sp' hm; unfold sllMoveSp in hm.
+    dms; tc; subst; inv hm; auto.
+  Qed.
+
+  Lemma sllMoveSp_preserves_lhss_invar :
+    forall rm a sp sp',
+      sll_sp_lhss_from_keyset rm sp
+      -> sllMoveSp a sp = MoveSucc sp'
+      -> sll_sp_lhss_from_keyset rm sp'.
+  Proof.
+    intros rm a sp sp' hk hm.
+    unfold sllMoveSp in hm; dms; tc; inv hm; sis.
+    eapply sll_consume_preserves_keyset_invar; eauto.
+  Qed.
+
+  Definition sllMove (a : terminal) (sps : list sll_subparser) : move_result sll_subparser :=
+    aggrMoveResults (map (sllMoveSp a) sps).
+
+  Lemma sllMove_preserves_prediction :
+    forall t sp' sps sps',
+      sllMove t sps = inr sps'
+      -> In sp' sps'
+      -> exists sp, In sp sps /\ sp'.(sll_prediction) = sp.(sll_prediction).
+  Proof.
+    intros t sp' sps sps' hm hi.
+    unfold move in hm.
+    eapply aggrMoveResults_succ_in_input in hm; eauto.
+    eapply in_map_iff in hm; destruct hm as [sp [hmsp hi']].
+    eexists; split; eauto.
+    eapply sllMoveSp_preserves_prediction; eauto.
+  Qed.
+
+  Lemma sllMove_preserves_lhss_invar :
+    forall rm a sps sps',
+      all_sll_sp_lhss_from_keyset rm sps
+      -> sllMove a sps = inr sps'
+      -> all_sll_sp_lhss_from_keyset rm sps'.
+  Proof.
+    intros rm a sps sps' hk hm sp' hi'.
+    eapply aggrMoveResults_map_backwards in hm; eauto.
+    destruct hm as [sp [hi hm]].
+    eapply sllMoveSp_preserves_lhss_invar; eauto.
+  Qed.
 
   (* closure operation *)
 
-Definition sll_cstep (rm : rhs_map) (vi : NtSet.t) (sp : sll_subparser) : 
+  Definition simReturn (cm : closure_map) (sp : sll_subparser) : option (list sll_subparser) :=
+    match sp with
+    | SllSp pred (SF (Some x) [], []) =>
+      let dsts := destFrames (SF (Some x) []) cm in
+      let sps' := map (fun d => SllSp pred (d, [])) dsts
+      in  Some sps'
+    | _ => None
+    end.
+
+  Lemma simReturn_preserves_prediction :
+    forall cm sp sp' sps',
+      simReturn cm sp = Some sps'
+      -> In sp' sps'
+      -> sll_prediction sp' = sll_prediction sp.
+  Proof.
+    intros cm [pred (fr, frs)] sp' sps' hs hi; sis; dms; tc; inv hs.
+    apply in_map_iff in hi; destruct hi as [? [? ?]]; subst; auto.
+  Qed.
+
+  Lemma simReturn_stack_shape :
+    forall cm sp sps',
+      simReturn cm sp = Some sps'
+      -> exists x, sll_stack sp = (SF (Some x) [], []).
+  Proof.
+    intros cm sp sps' hr; unfold simReturn in hr; dms; inv hr; sis; eauto.
+  Qed.
+
+  Lemma simReturn_lhss_invar :
+    forall pm cm sp sps',
+      simReturn cm sp = Some sps'
+      -> all_sll_sp_lhss_from_keyset pm sps'.
+  Proof.
+    intros pm cm [pred (fr, frs)] sps' hr sp' hi; sis; dms; tc; inv hr.
+    apply in_map_iff in hi; destruct hi as [[o suf] [heq hi]]; subst. 
+    repeat red; auto.
+  Qed.
+
+  Definition sllCstep (rm : rhs_map) (vi : NtSet.t) (sp : sll_subparser) : 
     subparser_closure_step_result :=
     match sp with
     | SllSp pred (fr, frs) =>
       match fr, frs with
+      | SF _ [], [] => CstepDone
       (* return to caller frame *)
       | SF (Some x) [], SF o_cr suf_cr :: frs_tl =>
         let stk':= (SF o_cr suf_cr, frs_tl) 
         in  CstepK (NtSet.remove x vi) [SllSp pred stk']
       (* done case -- top stack symbol is a terminal *)
-      | SF (Some _) (T _ :: _), _ => CstepDone
+      | SF _ (T _ :: _), _ => CstepDone
       (* push case *)
       | SF o (NT x :: suf), _ =>
         if NtSet.mem x vi then
@@ -62,19 +143,53 @@ Definition sll_cstep (rm : rhs_map) (vi : NtSet.t) (sp : sll_subparser) :
       | _, _ => CstepError SpInvalidState
       end
     end.
+  
+  Lemma sllCstep_preserves_prediction :
+    forall rm sp sp' sps' vi vi',
+      sllCstep rm vi sp = CstepK vi' sps'
+      -> In sp' sps'
+      -> sp.(sll_prediction) = sp'.(sll_prediction).
+  Proof.
+    intros rm sp sp' sps' vi vi' hs hi.
+    unfold sllCstep in hs; dms; tc; inv hs; try solve [inv hi].
+    - apply in_singleton_eq in hi; subst; auto.
+    - apply in_map_iff in hi.
+      destruct hi as [rhs [heq hi]]; subst; auto.
+    - apply in_map_iff in hi.
+      destruct hi as [rhs [heq hi]]; subst; auto.
+  Qed.
 
-  Lemma cstep_meas_lt :
+  Lemma sllCstep_preserves_lhss_invar :
+    forall rm vi sp vi' sp' sps',
+      sll_sp_lhss_from_keyset rm sp
+      -> sllCstep rm vi sp = CstepK vi' sps'
+      -> In sp' sps'
+      -> sll_sp_lhss_from_keyset rm sp'.
+  Proof.
+    intros rm vi sp vi' sp' sps' hk hs hi.
+    unfold sllCstep in hs; dms; tc; inv hs; red; try solve [inv hi].
+    - apply in_singleton_eq in hi; subst.
+      eapply sll_return_preserves_keyset_invar; eauto.
+    - apply in_map_iff in hi; destruct hi as [rhs [heq hi]]; subst.
+      eapply sll_push_preserves_keyset_invar; eauto.
+      eapply rhssFor_keySet; eauto.
+    - apply in_map_iff in hi; destruct hi as [rhs [heq hi]]; subst.
+      eapply sll_push_preserves_keyset_invar; eauto.
+      eapply rhssFor_keySet; eauto.
+  Qed.
+
+  Lemma sllCstep_meas_lt :
     forall (rm     : rhs_map)
            (sp sp' : sll_subparser)
            (sps'   : list sll_subparser)
            (vi vi' : NtSet.t),
       sll_sp_lhss_from_keyset rm sp
-      -> sll_cstep rm vi sp = CstepK vi' sps'
+      -> sllCstep rm vi sp = CstepK vi' sps'
       -> In sp' sps'
       -> lex_nat_pair (sll_meas rm vi' sp') (sll_meas rm vi sp).
   Proof.
     intros rm sp sp' sps' vi vi' ha hs hi. 
-    unfold sll_cstep in hs; dmeqs h; tc; inv hs; try solve [inv hi].
+    unfold sllCstep in hs; dmeqs h; tc; inv hs; try solve [inv hi].
     - apply in_singleton_eq in hi; subst.
       eapply sll_meas_lt_after_return; eauto.
     - apply in_map_iff in hi.
@@ -91,204 +206,204 @@ Definition sll_cstep (rm : rhs_map) (vi : NtSet.t) (sp : sll_subparser) :
       + eapply rhssFor_allRhss; eauto.
   Defined.
 
-  Lemma acc_after_step :
-    forall pm sp sp' sps' vi vi',
-      sp_pushes_from_keyset pm sp
-      -> cstep pm vi sp = CstepK vi' sps'
+  Lemma acc_after_sll_step :
+    forall rm sp sp' sps' vi vi',
+      sll_sp_lhss_from_keyset rm sp
+      -> sllCstep rm vi sp = CstepK vi' sps'
       -> In sp' sps'
-      -> Acc lex_nat_pair (meas pm vi sp)
-      -> Acc lex_nat_pair (meas pm vi' sp').
+      -> Acc lex_nat_pair (sll_meas rm vi sp)
+      -> Acc lex_nat_pair (sll_meas rm vi' sp').
   Proof.
-    intros pm sp sp' sps' vi vi' hk heq hi ha.
+    intros rm sp sp' sps' vi vi' hk heq hi ha.
     eapply Acc_inv; eauto.
-    eapply cstep_meas_lt; eauto.
+    eapply sllCstep_meas_lt; eauto.
   Defined.
   
-  Fixpoint sllc (rm : production_map)
+  Fixpoint sllc (rm : rhs_map)
                 (cm : closure_map)
                 (vi : NtSet.t)
-                (sp : subparser)
-                (hk : sp_pushes_from_keyset pm sp)
-                (a  : Acc lex_nat_pair (meas pm vi sp))
-    : closure_result :=
+                (sp : sll_subparser)
+                (hk : sll_sp_lhss_from_keyset rm sp)
+                (a  : Acc lex_nat_pair (sll_meas rm vi sp))
+    : closure_result sll_subparser :=
     match simReturn cm sp with
     | Some sps' => inr sps'
     | None      =>
-      match cstep pm vi sp as r return cstep pm vi sp = r -> _ with
+      match sllCstep rm vi sp as r return sllCstep rm vi sp = r -> _ with
       | CstepDone       => fun _  => inr [sp]
       | CstepError e    => fun _  => inl e
       | CstepK vi' sps' => 
         fun hs => 
           let crs := dmap sps' (fun sp' hi =>
-                                  sllc pm cm vi' sp'
-                                       (cstep_preserves_pfk _ _ _ _ _ _ hk hs hi)
-                                       (acc_after_step _ _ _ _ _ _ hk hs hi a))
+                                  sllc rm cm vi' sp'
+                                       (sllCstep_preserves_lhss_invar _ _ _ _ _ _ hk hs hi)
+                                       (acc_after_sll_step _ _ _ _ _ _ hk hs hi a))
           in  aggrClosureResults crs
       end eq_refl
     end.
 
   Lemma sllc_unfold :
-    forall pm cm vi sp hk a,
-      sllc pm cm vi sp hk a =
+    forall rm cm vi sp hk a,
+      sllc rm cm vi sp hk a =
       match simReturn cm sp with
       | Some sps' => inr sps'
       | None      =>
-        match cstep pm vi sp as r return cstep pm vi sp = r -> _ with
+        match sllCstep rm vi sp as r return sllCstep rm vi sp = r -> _ with
         | CstepDone       => fun _  => inr [sp]
         | CstepError e    => fun _  => inl e
         | CstepK vi' sps' => 
           fun hs => 
             let crs := dmap sps' (fun sp' hi =>
-                                    sllc pm cm vi' sp'
-                                         (cstep_preserves_pfk _ _ _ _ _ _ hk hs hi)
-                                          (acc_after_step _ _ _ _ _ _ hk hs hi a))
+                                    sllc rm cm vi' sp'
+                                         (sllCstep_preserves_lhss_invar _ _ _ _ _ _ hk hs hi)
+                                          (acc_after_sll_step _ _ _ _ _ _ hk hs hi a))
             in  aggrClosureResults crs
         end eq_refl
       end.
   Proof.
-    intros pm cm vi sp hk a; destruct a; auto.
+    intros rm cm vi sp hk a; destruct a; auto.
   Qed.
 
   Lemma sllc_cases' :
-    forall (pm  : production_map)
+    forall (rm  : rhs_map)
            (cm  : closure_map)
            (vi  : NtSet.t)
-           (sp  : subparser)
-           (hk  : sp_pushes_from_keyset pm sp)
-           (a   : Acc lex_nat_pair (meas pm vi sp))
+           (sp  : sll_subparser)
+           (hk  : sll_sp_lhss_from_keyset rm sp)
+           (a   : Acc lex_nat_pair (sll_meas rm vi sp))
            (sr  : subparser_closure_step_result)
-           (cr  : closure_result)
-           (heq : cstep pm vi sp = sr),
+           (cr  : closure_result sll_subparser)
+           (heq : sllCstep rm vi sp = sr),
       match simReturn cm sp with
       | Some sps' => inr sps'
       | None      =>
-        match sr as r return cstep pm vi sp = r -> closure_result with
+        match sr as r return sllCstep rm vi sp = r -> closure_result sll_subparser with
         | CstepDone       => fun _  => inr [sp]
         | CstepError e    => fun _  => inl e
         | CstepK vi' sps' => 
           fun hs => 
-            let crs := dmap sps' (fun sp' hi => sllc pm cm vi' sp'
-                                                     (cstep_preserves_pfk _ _ _ _ _ _ hk hs hi)
-                                                       (acc_after_step _ _ _ _ _ _ hk hs hi a))
+            let crs := dmap sps' (fun sp' hi => sllc rm cm vi' sp'
+                                                     (sllCstep_preserves_lhss_invar _ _ _ _ _ _ hk hs hi)
+                                                       (acc_after_sll_step _ _ _ _ _ _ hk hs hi a))
             in  aggrClosureResults crs
         end heq
       end = cr
       -> match cr with
          | inl e => 
            sr = CstepError e
-           \/ exists (sps : list subparser)
+           \/ exists (sps : list sll_subparser)
                      (vi' : NtSet.t)
-                     (hs  : cstep pm vi sp = CstepK vi' sps)
-                     (crs : list closure_result),
+                     (hs  : sllCstep rm vi sp = CstepK vi' sps)
+                     (crs : list (closure_result sll_subparser)),
                crs = dmap sps (fun sp' hi => 
-                                 sllc pm cm vi' sp'
-                                      (cstep_preserves_pfk _ _ _ _ _ _ hk hs hi)
-                                       (acc_after_step _ _ _ _ _ _ hk hs hi a))
+                                 sllc rm cm vi' sp'
+                                      (sllCstep_preserves_lhss_invar _ _ _ _ _ _ hk hs hi)
+                                       (acc_after_sll_step _ _ _ _ _ _ hk hs hi a))
                /\ aggrClosureResults crs = inl e
          | inr sps =>
            simReturn cm sp = Some sps
            \/ simReturn cm sp = None
               /\ ((sr = CstepDone /\ sps = [sp])
-                  \/ exists (sps' : list subparser)
+                  \/ exists (sps' : list sll_subparser)
                             (vi'  : NtSet.t)
-                            (hs   : cstep pm vi sp = CstepK vi' sps')
-                            (crs  : list closure_result),
+                            (hs   : sllCstep rm vi sp = CstepK vi' sps')
+                            (crs  : list (closure_result sll_subparser)),
                      crs = dmap sps' (fun sp' hi => 
-                                        sllc pm cm vi' sp'
-                                             (cstep_preserves_pfk _ _ _ _ _ _ hk hs hi)
-                                             (acc_after_step _ _ _ _ _ _ hk hs hi a))
+                                        sllc rm cm vi' sp'
+                                             (sllCstep_preserves_lhss_invar _ _ _ _ _ _ hk hs hi)
+                                             (acc_after_sll_step _ _ _ _ _ _ hk hs hi a))
                      /\ aggrClosureResults crs = inr sps)
          end.
   Proof.
-    intros pm cm vi sp hk a sr cr heq.
+    intros rm cm vi sp hk a sr cr heq.
     dms; tc; intros heq'; try solve [inv heq'; eauto | eauto 10].
   Qed.
   
   Lemma sllc_cases :
-    forall (pm : production_map)
+    forall (rm : rhs_map)
            (cm : closure_map)
-           (sp : subparser)
+           (sp : sll_subparser)
            (vi : NtSet.t)
-           (hk : sp_pushes_from_keyset pm sp)
-           (a  : Acc lex_nat_pair (meas pm vi sp))
-           (cr : closure_result),
-      sllc pm cm vi sp hk a = cr
+           (hk : sll_sp_lhss_from_keyset rm sp)
+           (a  : Acc lex_nat_pair (sll_meas rm vi sp))
+           (cr : closure_result sll_subparser),
+      sllc rm cm vi sp hk a = cr
       -> match cr with
          | inl e => 
-           cstep pm vi sp = CstepError e
-           \/ exists (sps : list subparser)
+           sllCstep rm vi sp = CstepError e
+           \/ exists (sps : list sll_subparser)
                      (vi' : NtSet.t)
-                     (hs  : cstep pm vi sp = CstepK vi' sps)
-                     (crs : list closure_result),
+                     (hs  : sllCstep rm vi sp = CstepK vi' sps)
+                     (crs : list (closure_result sll_subparser)),
                crs = dmap sps (fun sp' hi => 
-                                 sllc pm cm vi' sp'
-                                      (cstep_preserves_pfk _ _ _ _ _ _ hk hs hi)
-                                   (acc_after_step _ _ _ _ _ _ hk hs hi a))
+                                 sllc rm cm vi' sp'
+                                      (sllCstep_preserves_lhss_invar _ _ _ _ _ _ hk hs hi)
+                                   (acc_after_sll_step _ _ _ _ _ _ hk hs hi a))
                /\ aggrClosureResults crs = inl e
          | inr sps =>
            simReturn cm sp = Some sps
            \/ simReturn cm sp = None
-              /\ ((cstep pm vi sp = CstepDone /\ sps = [sp])
-                  \/ exists (sps' : list subparser)
+              /\ ((sllCstep rm vi sp = CstepDone /\ sps = [sp])
+                  \/ exists (sps' : list sll_subparser)
                             (vi'  : NtSet.t)
-                            (hs   : cstep pm vi sp = CstepK vi' sps')
-                            (crs  : list closure_result),
+                            (hs   : sllCstep rm vi sp = CstepK vi' sps')
+                            (crs  : list (closure_result sll_subparser)),
                      crs = dmap sps' (fun sp' hi => 
-                                        sllc pm cm vi' sp'
-                                             (cstep_preserves_pfk _ _ _ _ _ _ hk hs hi)
-                                             (acc_after_step _ _ _ _ _ _ hk hs hi a))
+                                        sllc rm cm vi' sp'
+                                             (sllCstep_preserves_lhss_invar _ _ _ _ _ _ hk hs hi)
+                                             (acc_after_sll_step _ _ _ _ _ _ hk hs hi a))
                      /\ aggrClosureResults crs = inr sps)
                   end.
   Proof.
-    intros pm cm vi sp hk a cr hs; subst.
+    intros rm cm vi sp hk a cr hs; subst.
     rewrite sllc_unfold.
     eapply sllc_cases'; eauto.
   Qed.
 
   Lemma sllc_success_cases :
-    forall pm cm vi sp hk a sps,
-      sllc pm cm vi sp hk a = inr sps
+    forall rm cm vi sp hk a sps,
+      sllc rm cm vi sp hk a = inr sps
       -> simReturn cm sp = Some sps
          \/ simReturn cm sp = None
-            /\ ((cstep pm vi sp = CstepDone /\ sps = [sp])
-                \/ exists (sps' : list subparser)
+            /\ ((sllCstep rm vi sp = CstepDone /\ sps = [sp])
+                \/ exists (sps' : list sll_subparser)
                           (vi'  : NtSet.t)
-                          (hs   : cstep pm vi sp = CstepK vi' sps')
-                          (crs  : list closure_result),
+                          (hs   : sllCstep rm vi sp = CstepK vi' sps')
+                          (crs  : list (closure_result sll_subparser)),
                    crs = dmap sps' (fun sp' hi => 
-                                      sllc pm cm vi' sp'
-                                           (cstep_preserves_pfk _ _ _ _ _ _ hk hs hi)
-                                           (acc_after_step _ _ _ _ _ _ hk hs hi a))
+                                      sllc rm cm vi' sp'
+                                           (sllCstep_preserves_lhss_invar _ _ _ _ _ _ hk hs hi)
+                                           (acc_after_sll_step _ _ _ _ _ _ hk hs hi a))
                    /\ aggrClosureResults crs = inr sps).
   Proof.
     intros ? ? ? ? ? ? sps ?; apply sllc_cases with (cr := inr sps); auto.
   Qed.
 
   Lemma sllc_error_cases :
-    forall pm cm sp vi hk a e,
-      sllc pm cm vi sp hk a = inl e
-      -> cstep pm vi sp = CstepError e
-         \/ exists (sps : list subparser)
+    forall rm cm sp vi hk a e,
+      sllc rm cm vi sp hk a = inl e
+      -> sllCstep rm vi sp = CstepError e
+         \/ exists (sps : list sll_subparser)
                    (vi' : NtSet.t)
-                   (hs  : cstep pm vi sp = CstepK vi' sps)
-                   (crs : list closure_result),
+                   (hs  : sllCstep rm vi sp = CstepK vi' sps)
+                   (crs : list (closure_result sll_subparser)),
           crs = dmap sps (fun sp' hi => 
-                            sllc pm cm vi' sp'
-                                 (cstep_preserves_pfk _ _ _ _ _ _ hk hs hi)
-                                 (acc_after_step _ _ _ _ _ _ hk hs hi a))
+                            sllc rm cm vi' sp'
+                                 (sllCstep_preserves_lhss_invar _ _ _ _ _ _ hk hs hi)
+                                 (acc_after_sll_step _ _ _ _ _ _ hk hs hi a))
           /\ aggrClosureResults crs = inl e.
   Proof.
-    intros pm cm sp vi hk a e hs; apply sllc_cases with (cr := inl e); auto.
+    intros rm cm sp vi hk a e hs; apply sllc_cases with (cr := inl e); auto.
   Qed.
 
-    Lemma sllc_preserves_prediction' :
-    forall pm cm pair (a : Acc lex_nat_pair pair) vi sp sp' sps' hk a',
-      pair = meas pm vi sp
-      -> sllc pm cm vi sp hk a' = inr sps'
+  Lemma sllc_preserves_prediction' :
+    forall rm cm pair (a : Acc lex_nat_pair pair) vi sp sp' sps' hk a',
+      pair = sll_meas rm vi sp
+      -> sllc rm cm vi sp hk a' = inr sps'
       -> In sp' sps'
-      -> sp'.(prediction) = sp.(prediction).
+      -> sp'.(sll_prediction) = sp.(sll_prediction).
   Proof.
-    intros pm cm pair a.
+    intros rm cm pair a.
     induction a as [pair hlt IH]; intros vi sp sp' sps' hk a' heq hs hi; subst.
     apply sllc_success_cases in hs.
     destruct hs as [hr | [hr [[hs heq] | [sps'' [av' [hs [crs [heq heq']]]]]]]]; subst.
@@ -300,67 +415,67 @@ Definition sll_cstep (rm : rhs_map) (vi : NtSet.t) (sp : sll_subparser) :
       eapply dmap_in in hi'; eauto.
       destruct hi' as [sp'' [hi''' [_ heq]]].
       eapply IH in heq; subst; eauto.
-      + apply cstep_preserves_prediction with (sp' := sp'') in hs; auto.
+      + apply sllCstep_preserves_prediction with (sp' := sp'') in hs; auto.
         rewrite hs; auto.
-      + eapply cstep_meas_lt; eauto.
+      + eapply sllCstep_meas_lt; eauto.
   Qed.
 
   Lemma sllc_preserves_prediction :
-    forall pm cm vi sp sp' sps' hk (a : Acc lex_nat_pair (meas pm vi sp)),
-      sllc pm cm vi sp hk a = inr sps'
+    forall rm cm vi sp sp' sps' hk (a : Acc lex_nat_pair (sll_meas rm vi sp)),
+      sllc rm cm vi sp hk a = inr sps'
       -> In sp' sps'
-      -> sp'.(prediction) = sp.(prediction).
+      -> sp'.(sll_prediction) = sp.(sll_prediction).
   Proof.
     intros; eapply sllc_preserves_prediction'; eauto.
   Qed.
 
-  Lemma sllc_preserves_push_invar' :
-    forall pm cm pair (ha : Acc lex_nat_pair pair) vi sp hk ha' sps',
-      pair = meas pm vi sp
-      -> sllc pm cm vi sp hk ha' = inr sps'
-      -> all_sp_pushes_from_keyset pm sps'.
+  Lemma sllc_preserves_lhss_invar' :
+    forall rm cm pair (ha : Acc lex_nat_pair pair) vi sp hk ha' sps',
+      pair = sll_meas rm vi sp
+      -> sllc rm cm vi sp hk ha' = inr sps'
+      -> all_sll_sp_lhss_from_keyset rm sps'.
   Proof.
-    intros pm cm pair a.
+    intros rm cm pair a.
     induction a as [pair hlt IH].
     intros vi sp hk ha' sps'' heq hc; subst.
     pose proof hc as hc'; apply sllc_success_cases in hc.
     destruct hc as [hr | [hr [[hc heq] | [sps' [vi' [hc [crs [heq heq']]]]]]]]; subst; intros sp''' hi.
-    - eapply simReturn_push_invar; eauto. 
+    - eapply simReturn_lhss_invar; eauto. 
     - apply in_singleton_eq in hi; subst; auto.
     - eapply aggrClosureResults_succ_in_input in heq'; eauto.
       destruct heq' as [sps [hi' hi'']].
       eapply dmap_in in hi'; eauto.
       destruct hi' as [sp'' [hi''' [_ heq]]].
       eapply IH in heq; subst; eauto.
-      eapply cstep_meas_lt; eauto.
+      eapply sllCstep_meas_lt; eauto.
   Qed.
 
-  Lemma sllc_preserves_push_invar :
-    forall pm cm vi sp sps' hk ha,
-      sllc pm cm vi sp hk ha = inr sps'
-      -> sp_pushes_from_keyset pm sp
-      -> all_sp_pushes_from_keyset pm sps'.
+  Lemma sllc_preserves_lhss_invar :
+    forall rm cm vi sp sps' hk ha,
+      sllc rm cm vi sp hk ha = inr sps'
+      -> sll_sp_lhss_from_keyset rm sp
+      -> all_sll_sp_lhss_from_keyset rm sps'.
   Proof.
-    intros; eapply sllc_preserves_push_invar'; eauto.
+    intros; eapply sllc_preserves_lhss_invar'; eauto.
   Qed.
 
-  Definition sllClosure (pm  : production_map)
+  Definition sllClosure (rm  : rhs_map)
                         (cm  : closure_map)
-                        (sps : list subparser)
-                        (hk  : all_sp_pushes_from_keyset pm sps) :
-                        sum prediction_error (list subparser) :=
+                        (sps : list sll_subparser)
+                        (hk  : all_sll_sp_lhss_from_keyset rm sps) :
+                        sum prediction_error (list sll_subparser) :=
     aggrClosureResults (dmap sps (fun sp hi =>
-                                    sllc pm cm NtSet.empty sp
-                                         (pfk_list__pfk_mem _ _ sp hk hi)
+                                    sllc rm cm NtSet.empty sp
+                                         (sll_ulk_list__ulk_mem _ _ sp hk hi)
                                          (lex_nat_pair_wf _))).
 
   Lemma sllClosure_preserves_prediction :
-    forall pm cm sps hk sp' sps',
-      sllClosure pm cm sps hk = inr sps'
+    forall rm cm sps hk sp' sps',
+      sllClosure rm cm sps hk = inr sps'
       -> In sp' sps'
-      -> exists sp, In sp sps /\ prediction sp' = prediction sp.
+      -> exists sp, In sp sps /\ sll_prediction sp' = sll_prediction sp.
   Proof.
-    intros pm cm sps hk sp' sps' hc hi.
+    intros rm cm sps hk sp' sps' hc hi.
     eapply aggrClosureResults_succ_in_input in hc; eauto.
     destruct hc as [sps'' [hi' hi'']].
     eapply dmap_in in hi'; eauto; sis.
@@ -369,35 +484,35 @@ Definition sll_cstep (rm : rhs_map) (vi : NtSet.t) (sp : sll_subparser) :
     eapply sllc_preserves_prediction; eauto.
   Qed.
 
-  Lemma sllClosure_preserves_push_invar :
-    forall pm cm sps hk sps',
-      sllClosure pm cm sps hk = inr sps'
-      -> all_sp_pushes_from_keyset pm sps
-      -> all_sp_pushes_from_keyset pm sps'.
+  Lemma sllClosure_preserves_lhss_invar :
+    forall rm cm sps hk sps',
+      sllClosure rm cm sps hk = inr sps'
+      -> all_sll_sp_lhss_from_keyset rm sps
+      -> all_sll_sp_lhss_from_keyset rm sps'.
   Proof.
-    intros pm cm sps hk sps'' hc ha sp' hi.
+    intros rm cm sps hk sps'' hc ha sp' hi.
     eapply aggrClosureResults_succ_in_input in hc; eauto.
     destruct hc as [sps' [hi' hi'']].
     eapply dmap_in with (l := sps) in hi'; eauto; sis.
     destruct hi' as [sp [? [hi''' hspc]]].
-    eapply sllc_preserves_push_invar; eauto.
+    eapply sllc_preserves_lhss_invar; eauto.
   Qed.
 
-  Module Subparser_as_UOT <: UsualOrderedType.
+  Module SLL_Subparser_as_UOT <: UsualOrderedType.
 
     Module L := List_as_UOT SF_as_UOT.
     Module P := Pair_as_UOT Gamma_as_UOT L.
 
-    Definition t := subparser.
+    Definition t := sll_subparser.
 
     Definition eq       := @eq t.
     Definition eq_refl  := @eq_refl t.
     Definition eq_sym   := @eq_sym t.
     Definition eq_trans := @eq_trans t.
 
-    Definition lt (x y : subparser) : Prop :=
+    Definition lt (x y : sll_subparser) : Prop :=
       match x, y with
-      | Sp pred (fr, frs), Sp pred' (fr', frs') =>
+      | SllSp pred (fr, frs), SllSp pred' (fr', frs') =>
         P.lt (pred, fr :: frs) (pred', fr' :: frs')
       end.
 
@@ -416,9 +531,9 @@ Definition sll_cstep (rm : rhs_map) (vi : NtSet.t) (sp : sll_subparser) :
       eapply P.lt_not_eq; eauto.
     Qed.
 
-    Definition compare (x y : subparser) : Compare lt eq x y.
+    Definition compare (x y : sll_subparser) : Compare lt eq x y.
       refine (match x, y with
-              | Sp pred (fr, frs), Sp pred' (fr', frs') =>
+              | SllSp pred (fr, frs), SllSp pred' (fr', frs') =>
                 match P.compare (pred, fr :: frs) (pred', fr' :: frs') with
                 | LT hl => LT _
                 | GT he => GT _
@@ -427,9 +542,9 @@ Definition sll_cstep (rm : rhs_map) (vi : NtSet.t) (sp : sll_subparser) :
               end); red; tc.
     Defined.
 
-    Definition eq_dec (x y : subparser) : {x = y} + {x <> y}.
+    Definition eq_dec (x y : sll_subparser) : {x = y} + {x <> y}.
       refine (match x, y with
-              | Sp pred (fr, frs), Sp pred' (fr', frs') =>
+              | SllSp pred (fr, frs), SllSp pred' (fr', frs') =>
                 match P.eq_dec (pred, fr :: frs) (pred', fr' :: frs') with
                 | left he  => left _
                 | right hn => right _
@@ -437,17 +552,18 @@ Definition sll_cstep (rm : rhs_map) (vi : NtSet.t) (sp : sll_subparser) :
               end); tc.
     Defined.
 
-  End Subparser_as_UOT.
+  End SLL_Subparser_as_UOT.
 
-  Module SpSet := FSetList.Make Subparser_as_UOT.
-  Definition setify (sps : list subparser) : SpSet.t :=
-    fold_right SpSet.add SpSet.empty sps.
+  Module SllSpSet := FSetList.Make SLL_Subparser_as_UOT.
+
+  Definition setify (sps : list sll_subparser) : SllSpSet.t :=
+    fold_right SllSpSet.add SllSpSet.empty sps.
   
-  Definition cache_key := (list subparser * terminal)%type.
+  Definition cache_key := (list sll_subparser * terminal)%type.
 
   Module CacheKey_as_UOT <: UsualOrderedType.
 
-    Module L := List_as_UOT Subparser_as_UOT.
+    Module L := List_as_UOT SLL_Subparser_as_UOT.
     Module P := Pair_as_UOT L T_as_UOT.
 
     Definition t := cache_key.
@@ -489,157 +605,218 @@ Definition sll_cstep (rm : rhs_map) (vi : NtSet.t) (sp : sll_subparser) :
   
   (* A cache is a finite map with (list subparser * terminal) keys 
      and (list subparser) values *)
-  Definition cache : Type := Cache.t (list subparser).
+  Definition cache : Type := Cache.t (list sll_subparser).
 
-  Definition empty_cache : cache := Cache.empty (list subparser).
+  Definition empty_cache : cache := Cache.empty (list sll_subparser).
   
-  Definition sllTarget (pm  : production_map)
-                       (cm  : closure_map)
-                       (a   : terminal)
-                       (sps : list subparser)
-                       (hk  : all_sp_pushes_from_keyset pm sps) :
-                       sum prediction_error (list subparser) :=
-    match move a sps as m return move a sps = m -> _ with
+  Definition sllTarget (rm   : rhs_map)
+                       (cm   : closure_map)
+                       (a    : terminal)
+                       (sps  : list sll_subparser)
+                       (hk   : all_sll_sp_lhss_from_keyset rm sps) :
+                       sum prediction_error (list sll_subparser) :=
+    match sllMove a sps as m return sllMove a sps = m -> _ with
     | inl e    => fun _ => inl e
     | inr sps' =>
       fun hm =>
-        match sllClosure pm cm sps' (move_preserves_pfk pm a sps sps' hk hm) with
+        match sllClosure rm cm sps' (sllMove_preserves_lhss_invar rm a sps sps' hk hm) with
         | inl e     => inl e
         | inr sps'' => inr sps''
         end
     end eq_refl.
 
   Lemma sllTarget_cases' :
-    forall pm cm a sps hk mr (heq : move a sps = mr) tr,
-      match mr as m return move a sps = m -> _ with
+    forall rm cm a sps hk mr (heq : sllMove a sps = mr) tr,
+      match mr as m return sllMove a sps = m -> _ with
       | inl e    => fun _ => inl e
       | inr sps' =>
         fun hm =>
-          match sllClosure pm cm sps' (move_preserves_pfk pm a sps sps' hk hm) with
+          match sllClosure rm cm sps' (sllMove_preserves_lhss_invar rm a sps sps' hk hm) with
           | inl e     => inl e
           | inr sps'' => inr sps''
           end
       end heq = tr
       -> match tr with
          | inl e =>
-           move a sps = inl e
+           sllMove a sps = inl e
            \/ (exists sps' hk',
-                  move a sps = inr sps' /\ sllClosure pm cm sps' hk' = inl e) 
+                  sllMove a sps = inr sps' /\ sllClosure rm cm sps' hk' = inl e) 
          | inr sps'' =>
-           exists sps' hk', move a sps = inr sps'
-                            /\ sllClosure pm cm sps' hk' = inr sps''
+           exists sps' hk', sllMove a sps = inr sps'
+                            /\ sllClosure rm cm sps' hk' = inr sps''
          end.
   Proof.
-    intros pm cm a sps hk mr heq tr.
+    intros rm cm a sps hk mr heq tr.
     destruct mr as [e' | sps']; intros ?; subst; auto.
     destruct (sllClosure _ _ _ _) eqn:hc; eauto.
   Qed.
 
   Lemma sllTarget_cases :
-    forall pm cm a sps hk tr,
-      sllTarget pm cm a sps hk = tr
+    forall rm cm a sps hk tr,
+      sllTarget rm cm a sps hk = tr
       -> match tr with
          | inl e =>
-           move a sps = inl e
+           sllMove a sps = inl e
            \/ (exists sps' hk',
-                  move a sps = inr sps' /\ sllClosure pm cm sps' hk' = inl e) 
+                  sllMove a sps = inr sps' /\ sllClosure rm cm sps' hk' = inl e) 
          | inr sps'' =>
            (exists sps' hk',
-               move a sps = inr sps' /\ sllClosure pm cm sps' hk' = inr sps'')
+               sllMove a sps = inr sps' /\ sllClosure rm cm sps' hk' = inr sps'')
          end.
   Proof.
-    intros pm cm a sps hk tr ht; eapply sllTarget_cases'; eauto.
+    intros rm cm a sps hk tr ht; eapply sllTarget_cases'; eauto.
   Qed.
 
   Lemma sllTarget_preserves_prediction :
-    forall pm cm a sps hk sp' sps',
-      sllTarget pm cm a sps hk = inr sps'
+    forall rm cm a sps hk sp' sps',
+      sllTarget rm cm a sps hk = inr sps'
       -> In sp' sps'
-      -> exists sp, In sp sps /\ prediction sp = prediction sp'.
+      -> exists sp, In sp sps /\ sll_prediction sp = sll_prediction sp'.
   Proof.
-    intros pm cm a sps hk sp' sps'' hs hi.
+    intros rm cm a sps hk sp' sps'' hs hi.
     apply sllTarget_cases in hs.
     destruct hs as [sps' [hk' [hm hc]]].
     eapply sllClosure_preserves_prediction in hc; eauto.
     destruct hc as [sp'' [hi'' heq]]; rewrite heq.
-    eapply move_preserves_prediction in hm; eauto.
+    eapply sllMove_preserves_prediction in hm; eauto.
     destruct hm as [? [? ?]]; eauto.
   Qed.
 
-  Lemma sllTarget_preserves_push_invar :
-    forall pm cm a sps hk sps',
-      sllTarget pm cm a sps hk = inr sps'
-      -> all_sp_pushes_from_keyset pm sps
-      -> all_sp_pushes_from_keyset pm sps'.
+  Lemma sllTarget_preserves_lhss_invar :
+    forall rm cm a sps hk sps',
+      sllTarget rm cm a sps hk = inr sps'
+      -> all_sll_sp_lhss_from_keyset rm sps
+      -> all_sll_sp_lhss_from_keyset rm sps'.
   Proof.
-    intros pm cm a sps hk sps'' ht ha.
+    intros rm cm a sps hk sps'' ht ha.
     apply sllTarget_cases in ht.
     destruct ht as [sps' [hk' [hm hc]]].
-    eapply sllClosure_preserves_push_invar; eauto.
+    eapply sllClosure_preserves_lhss_invar; eauto.
   Qed.
 
-  Definition cache_stores_target_results pm cm ca :=
+  Definition cache_stores_target_results rm cm ca :=
     forall sps a sps',
       Cache.find (sps, a) ca = Some sps'
-      -> exists hk, sllTarget pm cm a sps hk = inr sps'.
+      -> exists hk, sllTarget rm cm a sps hk = inr sps'.
   
   Lemma sllTarget_add_preserves_cache_invar :
-    forall pm cm ca sps a sps' hk,
-      cache_stores_target_results pm cm ca
-      -> sllTarget pm cm a sps hk = inr sps'
-      -> cache_stores_target_results pm cm (Cache.add (sps, a) sps' ca).
+    forall rm cm ca sps a sps' hk,
+      cache_stores_target_results rm cm ca
+      -> sllTarget rm cm a sps hk = inr sps'
+      -> cache_stores_target_results rm cm (Cache.add (sps, a) sps' ca).
   Proof.
-    intros pm cm ca sps a sps' hk hc ht ka kb v hf.
+    intros rm cm ca sps a sps' hk hc ht ka kb v hf.
     destruct (CacheKey_as_UOT.eq_dec (ka, kb) (sps, a)) as [he | hn].
     - inv he; rewrite CacheFacts.add_eq_o in hf; inv hf; eauto.
     - rewrite CacheFacts.add_neq_o in hf; auto.
   Qed.
 
-  Lemma cache_lookup_preserves_push_invar :
-    forall pm cm sps a ca sps',
-      cache_stores_target_results pm cm ca
+  Lemma cache_lookup_preserves_lhss_invar :
+    forall rm cm sps a ca sps',
+      cache_stores_target_results rm cm ca
       -> Cache.find (sps, a) ca = Some sps'
-      -> all_sp_pushes_from_keyset pm sps'.
+      -> all_sll_sp_lhss_from_keyset rm sps'.
   Proof.
-    intros pm cm sps a ca sps' hc hf.
+    intros rm cm sps a ca sps' hc hf.
     apply hc in hf.
     destruct hf as [hk ht].
-    eapply sllTarget_preserves_push_invar; eauto.
+    eapply sllTarget_preserves_lhss_invar; eauto.
+  Qed.
+
+  Definition sllFinalConfig (sp : sll_subparser) : bool :=
+    match sp with
+    | SllSp _ (SF None [], []) => true
+    | _ => false
+    end.
+
+  Lemma sllFinalConfig_empty_stack :
+    forall sp pred stk,
+      sp = SllSp pred stk
+      -> sllFinalConfig sp = true
+      -> stk = (SF None [], []).
+  Proof.
+    intros sp pred stk ? hf; subst; unfold sllFinalConfig in hf; dms; tc.
+  Qed.
+
+  Definition sllAllPredictionsEqual (sp : sll_subparser) (sps : list sll_subparser) : bool :=
+    allEqual _ beqGamma sp.(sll_prediction) (map sll_prediction sps).
+
+  Definition sllHandleFinalSubparsers (sps : list sll_subparser) : prediction_result :=
+    match filter sllFinalConfig sps with
+    | []         => PredReject
+    | sp :: sps' => 
+      if sllAllPredictionsEqual sp sps' then
+        PredSucc sp.(sll_prediction)
+      else
+        PredAmbig sp.(sll_prediction)
+    end.
+
+  Lemma sllHandleFinalSubparsers_succ_facts :
+    forall sps rhs,
+      sllHandleFinalSubparsers sps = PredSucc rhs
+      -> exists sp o,
+        In sp sps
+        /\ sp.(sll_prediction) = rhs
+        /\ sp.(sll_stack) = (SF o [], []).
+  Proof.
+    intros sps rhs hh.
+    unfold sllHandleFinalSubparsers in hh.
+    destruct (filter _ _) as [| sp sps'] eqn:hf; tc.
+    destruct (sllAllPredictionsEqual _ _); tc; inv hh.
+    assert (hin : In sp (filter sllFinalConfig sps)).
+    { rewrite hf; apply in_eq. }
+    apply filter_In in hin.
+    destruct hin as [hin ht]; subst.
+    unfold sllFinalConfig in ht.
+    destruct sp as [pred ([o suf], frs)]; dms; tc.
+    repeat eexists; eauto.
+  Qed.
+
+  Lemma sllHandleFinalSubparsers_ambig_from_subparsers :
+    forall sps gamma,
+      sllHandleFinalSubparsers sps = PredAmbig gamma
+      -> exists sp, In sp sps /\ sp.(sll_prediction) = gamma.
+  Proof.
+    intros sps gamma hh.
+    unfold sllHandleFinalSubparsers in hh.
+    dmeqs h; tc; inv hh.
+    eexists; split; eauto.
+    eapply filter_cons_in; eauto.
   Qed.
   
-  Fixpoint sllPredict' (pm  : production_map)
+  Fixpoint sllPredict' (rm  : rhs_map)
                        (cm  : closure_map)
-                       (sps : list subparser)
+                       (sps : list sll_subparser)
                        (ts  : list token)
                        (ca  : cache)
-                       (hk  : all_sp_pushes_from_keyset pm sps)
-                       (hc  : cache_stores_target_results pm cm ca) :
+                       (hk  : all_sll_sp_lhss_from_keyset rm sps)
+                       (hc  : cache_stores_target_results rm cm ca) :
                        prediction_result * cache :=
     match ts with
-    | []            => (handleFinalSubparsers sps, ca)
-    | (a, l) :: ts' =>
+    | []            => (sllHandleFinalSubparsers sps, ca)
+    | @existT _ _ a _ :: ts' =>
       match sps with
       | []          => (PredReject, ca)
       | sp' :: sps' =>
-        if allPredictionsEqual sp' sps' then
-          (PredSucc sp'.(prediction), ca)
+        if sllAllPredictionsEqual sp' sps' then
+          (PredSucc sp'.(sll_prediction), ca)
         else
           match Cache.find (sps, a) ca as f
                 return Cache.find (sps, a) ca = f -> _ with 
           | Some sps'' =>
             fun hf =>
-               sllPredict' pm cm sps'' ts' ca
-                          (cache_lookup_preserves_push_invar _ _ _ _ _ _ hc hf) hc
+               sllPredict' rm cm sps'' ts' ca
+                          (cache_lookup_preserves_lhss_invar _ _ _ _ _ _ hc hf) hc
           | None =>
             fun _ =>
-              match sllTarget pm cm a sps hk as t
-                    return sllTarget pm cm a sps hk = t -> _ with
+              match sllTarget rm cm a sps hk as t
+                    return sllTarget rm cm a sps hk = t -> _ with
               | inl e     => fun _ => (PredError e, ca)
               | inr sps'' =>
                 fun ht => 
                   let ca' := Cache.add (sps, a) sps'' ca
-                  in  sllPredict' pm cm sps'' ts' ca'
-                                  (sllTarget_preserves_push_invar _ _ _ _ _ _ ht hk)
+                  in  sllPredict' rm cm sps'' ts' ca'
+                                  (sllTarget_preserves_lhss_invar _ _ _ _ _ _ ht hk)
                                   (sllTarget_add_preserves_cache_invar _ _ _ _ _ _ _ hc ht)
               end eq_refl
           end eq_refl
@@ -647,72 +824,72 @@ Definition sll_cstep (rm : rhs_map) (vi : NtSet.t) (sp : sll_subparser) :
     end.
 
   Lemma sllPredict'_cont_cases :
-    forall pm cm sps a ts' ca hk hc fr tr pr
+    forall rm cm sps a ts' ca hk hc fr tr pr
            (heq : Cache.find (sps, a) ca = fr)
-           (heq' : sllTarget pm cm a sps hk = tr),
+           (heq' : sllTarget rm cm a sps hk = tr),
       match fr as f return Cache.find (sps, a) ca = f -> _ with 
       | Some sps'' =>
         fun hf =>
-          sllPredict' pm cm sps'' ts' ca
-                      (cache_lookup_preserves_push_invar _ _ _ _ _ _ hc hf) hc
+          sllPredict' rm cm sps'' ts' ca
+                      (cache_lookup_preserves_lhss_invar _ _ _ _ _ _ hc hf) hc
       | None =>
         fun _ =>
-          match tr as t return sllTarget pm cm a sps hk = t -> _ with
+          match tr as t return sllTarget rm cm a sps hk = t -> _ with
           | inl e     => fun _ => (PredError e, ca)
           | inr sps'' =>
             fun ht => 
               let ca' := Cache.add (sps, a) sps'' ca
-              in  sllPredict' pm cm sps'' ts' ca'
-                              (sllTarget_preserves_push_invar _ _ _ _ _ _ ht hk)
+              in  sllPredict' rm cm sps'' ts' ca'
+                              (sllTarget_preserves_lhss_invar _ _ _ _ _ _ ht hk)
                               (sllTarget_add_preserves_cache_invar _ _ _ _ _ _ _ hc ht)
           end heq'
       end heq = pr
       -> match pr with
          | (PredSucc ys, ca') =>
            (exists sps'' (hf : Cache.find (sps, a) ca = Some sps''),
-               sllPredict' pm cm sps'' ts' ca
-                           (cache_lookup_preserves_push_invar _ _ _ _ _ _ hc hf) hc = (PredSucc ys, ca'))
-           \/ (exists sps'' (ht : sllTarget pm cm a sps hk = inr sps''),
-                  sllPredict' pm cm sps'' ts' (Cache.add (sps, a) sps'' ca)
-                              (sllTarget_preserves_push_invar _ _ _ _ _ _ ht hk)
+               sllPredict' rm cm sps'' ts' ca
+                           (cache_lookup_preserves_lhss_invar _ _ _ _ _ _ hc hf) hc = (PredSucc ys, ca'))
+           \/ (exists sps'' (ht : sllTarget rm cm a sps hk = inr sps''),
+                  sllPredict' rm cm sps'' ts' (Cache.add (sps, a) sps'' ca)
+                              (sllTarget_preserves_lhss_invar _ _ _ _ _ _ ht hk)
                               (sllTarget_add_preserves_cache_invar _ _ _ _ _ _ _ hc ht) = (PredSucc ys, ca'))
          | (PredAmbig ys, ca') =>
            (exists sps'' (hf : Cache.find (sps, a) ca = Some sps''),
-               sllPredict' pm cm sps'' ts' ca
-                           (cache_lookup_preserves_push_invar _ _ _ _ _ _ hc hf) hc = (PredAmbig ys, ca'))
-           \/ (exists sps'' (ht : sllTarget pm cm a sps hk = inr sps''),
-                  sllPredict' pm cm sps'' ts' (Cache.add (sps, a) sps'' ca)
-                              (sllTarget_preserves_push_invar _ _ _ _ _ _ ht hk)
+               sllPredict' rm cm sps'' ts' ca
+                           (cache_lookup_preserves_lhss_invar _ _ _ _ _ _ hc hf) hc = (PredAmbig ys, ca'))
+           \/ (exists sps'' (ht : sllTarget rm cm a sps hk = inr sps''),
+                  sllPredict' rm cm sps'' ts' (Cache.add (sps, a) sps'' ca)
+                              (sllTarget_preserves_lhss_invar _ _ _ _ _ _ ht hk)
                               (sllTarget_add_preserves_cache_invar _ _ _ _ _ _ _ hc ht) = (PredAmbig ys, ca'))
          | (PredReject, ca') =>
            (exists sps'' (hf : Cache.find (sps, a) ca = Some sps''),
-               sllPredict' pm cm sps'' ts' ca
-                           (cache_lookup_preserves_push_invar _ _ _ _ _ _ hc hf) hc = (PredReject, ca'))
-           \/ (exists sps'' (ht : sllTarget pm cm a sps hk = inr sps''),
-                  sllPredict' pm cm sps'' ts' (Cache.add (sps, a) sps'' ca)
-                              (sllTarget_preserves_push_invar _ _ _ _ _ _ ht hk)
+               sllPredict' rm cm sps'' ts' ca
+                           (cache_lookup_preserves_lhss_invar _ _ _ _ _ _ hc hf) hc = (PredReject, ca'))
+           \/ (exists sps'' (ht : sllTarget rm cm a sps hk = inr sps''),
+                  sllPredict' rm cm sps'' ts' (Cache.add (sps, a) sps'' ca)
+                              (sllTarget_preserves_lhss_invar _ _ _ _ _ _ ht hk)
                               (sllTarget_add_preserves_cache_invar _ _ _ _ _ _ _ hc ht) = (PredReject, ca'))
          | (PredError e, ca') =>
            (exists sps'' (hf : Cache.find (sps, a) ca = Some sps''),
-               sllPredict' pm cm sps'' ts' ca
-                           (cache_lookup_preserves_push_invar _ _ _ _ _ _ hc hf) hc = (PredError e, ca'))
-           \/ sllTarget pm cm a sps hk = inl e
-           \/ (exists sps'' (ht : sllTarget pm cm a sps hk = inr sps''),
-                  sllPredict' pm cm sps'' ts' (Cache.add (sps, a) sps'' ca)
-                              (sllTarget_preserves_push_invar _ _ _ _ _ _ ht hk)
+               sllPredict' rm cm sps'' ts' ca
+                           (cache_lookup_preserves_lhss_invar _ _ _ _ _ _ hc hf) hc = (PredError e, ca'))
+           \/ sllTarget rm cm a sps hk = inl e
+           \/ (exists sps'' (ht : sllTarget rm cm a sps hk = inr sps''),
+                  sllPredict' rm cm sps'' ts' (Cache.add (sps, a) sps'' ca)
+                              (sllTarget_preserves_lhss_invar _ _ _ _ _ _ ht hk)
                               (sllTarget_add_preserves_cache_invar _ _ _ _ _ _ _ hc ht) = (PredError e, ca'))
          end.
   Proof.
-    intros pm cm sps a ts' ca hk hc fr tr pr heq heq';
+    intros rm cm sps a ts' ca hk hc fr tr pr heq heq';
       dms; intros heq''; inv heq''; eauto.
   Qed.
 
   Lemma sllPredict'_succ_preserves_cache_invar :
-    forall pm cm ts sps ca hk hc ys ca',
-      sllPredict' pm cm sps ts ca hk hc = (PredSucc ys, ca')
-      -> cache_stores_target_results pm cm ca'.
+    forall rm cm ts sps ca hk hc ys ca',
+      sllPredict' rm cm sps ts ca hk hc = (PredSucc ys, ca')
+      -> cache_stores_target_results rm cm ca'.
   Proof.
-    intros pm cm ts; induction ts as [| (a,l) ts IH];
+    intros rm cm ts; induction ts as [| (a,l) ts IH];
       intros sps ca hk hc ys ca' hs; sis.
     - dms; tc; inv hs; auto.
     - dm; tc; dm; try solve [inv hs; auto].
@@ -721,14 +898,14 @@ Definition sll_cstep (rm : rhs_map) (vi : NtSet.t) (sp : sll_subparser) :
   Qed.
 
   Lemma sllPredict'_success_result_in_original_subparsers :
-    forall pm cm ts sps ca hk hc ys ca',
-      sllPredict' pm cm sps ts ca hk hc = (PredSucc ys, ca')
-      -> exists sp, In sp sps /\ sp.(prediction) = ys.
+    forall rm cm ts sps ca hk hc ys ca',
+      sllPredict' rm cm sps ts ca hk hc = (PredSucc ys, ca')
+      -> exists sp, In sp sps /\ sp.(sll_prediction) = ys.
   Proof.
-    intros pm cm ts. 
+    intros rm cm ts. 
     induction ts as [| (a,l) ts IH]; intros sps ca hk hc ys ca' hp; sis.
     - injection hp; intros _ hh. 
-      apply handleFinalSubparsers_succ_facts in hh.
+      apply sllHandleFinalSubparsers_succ_facts in hh.
       destruct hh as (sp' & _ & hi & heq & _); eauto.
     - destruct sps as [| sp' sps'] eqn:hs; tc; dmeq hall.
       + inv hp; exists sp'; split; auto; apply in_eq.
@@ -742,122 +919,122 @@ Definition sll_cstep (rm : rhs_map) (vi : NtSet.t) (sp : sll_subparser) :
           eapply sllTarget_preserves_prediction; eauto.
   Qed.
   
-  Definition sllInitSps (pm : production_map) (x : nonterminal) : list subparser :=
-    map (fun rhs => Sp rhs (SF (Some x) rhs, []))
-        (rhssFor x pm).
+  Definition sllInitSps (rm : rhs_map) (x : nonterminal) : list sll_subparser :=
+    map (fun rhs => SllSp rhs (SF (Some x) rhs, []))
+        (rhssFor x rm).
 
   Lemma sllInitSps_prediction_in_rhssFor :
-    forall pm x sp,
-      In sp (sllInitSps pm x)
-      -> In sp.(prediction) (rhssFor x pm).
+    forall rm x sp,
+      In sp (sllInitSps rm x)
+      -> In sp.(sll_prediction) (rhssFor x rm).
   Proof.
-    intros pm x sp hi; unfold sllInitSps in hi.
+    intros rm x sp hi; unfold sllInitSps in hi.
     apply in_map_iff in hi; firstorder; subst; auto.
   Qed.
 
-  Lemma sllInitSps_push_invar :
-    forall pm x,
-      all_sp_pushes_from_keyset pm (sllInitSps pm x).
+  Lemma sllInitSps_lhss_invar :
+    forall rm x,
+      all_sll_sp_lhss_from_keyset rm (sllInitSps rm x).
   Proof.
-    intros pm x sp hi.
+    intros rm x sp hi.
     apply in_map_iff in hi; destruct hi as [? [heq hi]]; subst.
     repeat red; auto.
   Qed.
 
-  Definition sllStartState (pm : production_map)
+  Definition sllStartState (rm : rhs_map)
                            (cm : closure_map)
                            (x  : nonterminal) :
-                           sum prediction_error (list subparser) :=
-    sllClosure pm cm (sllInitSps pm x) (sllInitSps_push_invar pm x).
+                           sum prediction_error (list sll_subparser) :=
+    sllClosure rm cm (sllInitSps rm x) (sllInitSps_lhss_invar rm x).
 
   Lemma sllStartState_sp_prediction_in_rhssFor :
-    forall pm cm x sp' sps',
-      sllStartState pm cm x = inr sps'
+    forall rm cm x sp' sps',
+      sllStartState rm cm x = inr sps'
       -> In sp' sps'
-      -> In sp'.(prediction) (rhssFor x pm).
+      -> In sp'.(sll_prediction) (rhssFor x rm).
   Proof.
-    intros pm cm x sp' sps' hs hi.
+    intros rm cm x sp' sps' hs hi.
     unfold sllStartState in hs.
     eapply sllClosure_preserves_prediction in hs; eauto.
     destruct hs as [sp [hi' heq]]; rewrite heq.
     apply sllInitSps_prediction_in_rhssFor; auto.
   Qed.
 
-  Lemma sllStartState_push_invar :
-    forall pm cm x sps,
-      sllStartState pm cm x = inr sps
-      -> all_sp_pushes_from_keyset pm sps.
+  Lemma sllStartState_lhss_invar :
+    forall rm cm x sps,
+      sllStartState rm cm x = inr sps
+      -> all_sll_sp_lhss_from_keyset rm sps.
   Proof.
-    intros pm cm x sps hs sp hi.
-    eapply sllClosure_preserves_push_invar; eauto.
-    apply sllInitSps_push_invar.
+    intros rm cm x sps hs sp hi.
+    eapply sllClosure_preserves_lhss_invar; eauto.
+    apply sllInitSps_lhss_invar.
   Qed.
   
-  Definition sllPredict (pm : production_map)
+  Definition sllPredict (rm : rhs_map)
                         (cm : closure_map)
                         (x  : nonterminal)
                         (ts : list token)
                         (ca : cache)
-                        (hc : cache_stores_target_results pm cm ca) :
+                        (hc : cache_stores_target_results rm cm ca) :
                         prediction_result * cache :=
-    match sllStartState pm cm x as s return sllStartState pm cm x = s -> _ with
+    match sllStartState rm cm x as s return sllStartState rm cm x = s -> _ with
     | inl msg => fun _  => (PredError msg, ca)
-    | inr sps => fun hs => sllPredict' pm cm sps ts ca (sllStartState_push_invar _ _ _ _ hs) hc
+    | inr sps => fun hs => sllPredict' rm cm sps ts ca (sllStartState_lhss_invar _ _ _ _ hs) hc
     end eq_refl.
 
   Lemma sllPredict_cases' :
-    forall pm cm x ts ca hc cr pr (heq : sllStartState pm cm x = cr),
-      match cr as s return sllStartState pm cm x = s -> _ with
+    forall rm cm x ts ca hc cr pr (heq : sllStartState rm cm x = cr),
+      match cr as s return sllStartState rm cm x = s -> _ with
       | inl msg => fun _  => (PredError msg, ca)
-      | inr sps => fun hs => sllPredict' pm cm sps ts ca (sllStartState_push_invar _ _ _ _ hs) hc
+      | inr sps => fun hs => sllPredict' rm cm sps ts ca (sllStartState_lhss_invar _ _ _ _ hs) hc
       end heq = pr
       -> match pr with
          | (PredSucc ys, ca') =>
-           (exists sps (hs : sllStartState pm cm x = inr sps),
-               sllPredict' pm cm sps ts ca (sllStartState_push_invar _ _ _ _ hs) hc = (PredSucc ys, ca'))
+           (exists sps (hs : sllStartState rm cm x = inr sps),
+               sllPredict' rm cm sps ts ca (sllStartState_lhss_invar _ _ _ _ hs) hc = (PredSucc ys, ca'))
          | (PredAmbig ys, ca') =>
-           (exists sps (hs : sllStartState pm cm x = inr sps),
-               sllPredict' pm cm sps ts ca (sllStartState_push_invar _ _ _ _ hs) hc = (PredAmbig ys, ca'))
+           (exists sps (hs : sllStartState rm cm x = inr sps),
+               sllPredict' rm cm sps ts ca (sllStartState_lhss_invar _ _ _ _ hs) hc = (PredAmbig ys, ca'))
          | (PredReject, ca') =>
-           (exists sps (hs : sllStartState pm cm x = inr sps),
-               sllPredict' pm cm sps ts ca (sllStartState_push_invar _ _ _ _ hs) hc = (PredReject, ca'))
+           (exists sps (hs : sllStartState rm cm x = inr sps),
+               sllPredict' rm cm sps ts ca (sllStartState_lhss_invar _ _ _ _ hs) hc = (PredReject, ca'))
          | (PredError e, ca') =>
-           sllStartState pm cm x = inl e
-           \/ (exists sps (hs : sllStartState pm cm x = inr sps),
-                  sllPredict' pm cm sps ts ca (sllStartState_push_invar _ _ _ _ hs) hc = (PredError e, ca'))
+           sllStartState rm cm x = inl e
+           \/ (exists sps (hs : sllStartState rm cm x = inr sps),
+                  sllPredict' rm cm sps ts ca (sllStartState_lhss_invar _ _ _ _ hs) hc = (PredError e, ca'))
          end.
   Proof.
-    intros pm cm x ts ca hc cr pr heq; dms; intros heq'; inv heq'; eauto.
+    intros rm cm x ts ca hc cr pr heq; dms; intros heq'; inv heq'; eauto.
   Qed.
 
   Lemma sllPredict_cases :
-    forall pm cm x ts ca hc pr,
-      sllPredict pm cm x ts ca hc = pr
+    forall rm cm x ts ca hc pr,
+      sllPredict rm cm x ts ca hc = pr
       -> match pr with
          | (PredSucc ys, ca') =>
-           (exists sps (hs : sllStartState pm cm x = inr sps),
-               sllPredict' pm cm sps ts ca (sllStartState_push_invar _ _ _ _ hs) hc = (PredSucc ys, ca'))
+           (exists sps (hs : sllStartState rm cm x = inr sps),
+               sllPredict' rm cm sps ts ca (sllStartState_lhss_invar _ _ _ _ hs) hc = (PredSucc ys, ca'))
          | (PredAmbig ys, ca') =>
-           (exists sps (hs : sllStartState pm cm x = inr sps),
-               sllPredict' pm cm sps ts ca (sllStartState_push_invar _ _ _ _ hs) hc = (PredAmbig ys, ca'))
+           (exists sps (hs : sllStartState rm cm x = inr sps),
+               sllPredict' rm cm sps ts ca (sllStartState_lhss_invar _ _ _ _ hs) hc = (PredAmbig ys, ca'))
          | (PredReject, ca') =>
-           (exists sps (hs : sllStartState pm cm x = inr sps),
-               sllPredict' pm cm sps ts ca (sllStartState_push_invar _ _ _ _ hs) hc = (PredReject, ca'))
+           (exists sps (hs : sllStartState rm cm x = inr sps),
+               sllPredict' rm cm sps ts ca (sllStartState_lhss_invar _ _ _ _ hs) hc = (PredReject, ca'))
          | (PredError e, ca') =>
-           sllStartState pm cm x = inl e
-           \/ (exists sps (hs : sllStartState pm cm x = inr sps),
-                  sllPredict' pm cm sps ts ca (sllStartState_push_invar _ _ _ _ hs) hc = (PredError e, ca'))
+           sllStartState rm cm x = inl e
+           \/ (exists sps (hs : sllStartState rm cm x = inr sps),
+                  sllPredict' rm cm sps ts ca (sllStartState_lhss_invar _ _ _ _ hs) hc = (PredError e, ca'))
          end.
   Proof.
     intros; eapply sllPredict_cases'; eauto.
   Qed.
 
   Lemma sllPredict_succ_in_rhssFor :
-    forall pm cm x ts ca hc ys ca',
-      sllPredict pm cm x ts ca hc = (PredSucc ys, ca')
-      -> In ys (rhssFor x pm).
+    forall rm cm x ts ca hc ys ca',
+      sllPredict rm cm x ts ca hc = (PredSucc ys, ca')
+      -> In ys (rhssFor x rm).
   Proof.
-    intros pm cm x ts ca hc ys ca' hs.
+    intros rm cm x ts ca hc ys ca' hs.
     apply sllPredict_cases in hs.
     destruct hs as [sps [hs hp]].
     eapply sllPredict'_success_result_in_original_subparsers in hp; eauto.
@@ -866,83 +1043,89 @@ Definition sll_cstep (rm : rhs_map) (vi : NtSet.t) (sp : sll_subparser) :
   Qed.
 
   Lemma sllPredict_succ_preserves_cache_invar :
-    forall pm cm x ts ca hc ys ca',
-      sllPredict pm cm x ts ca hc = (PredSucc ys, ca')
-      -> cache_stores_target_results pm cm ca'.
+    forall rm cm x ts ca hc ys ca',
+      sllPredict rm cm x ts ca hc = (PredSucc ys, ca')
+      -> cache_stores_target_results rm cm ca'.
   Proof.
-    intros pm cm x ts ca hc ys ca' hs.
+    intros rm cm x ts ca hc ys ca' hs.
     apply sllPredict_cases in hs.
     destruct hs as [sps [hs hp]].
     eapply sllPredict'_succ_preserves_cache_invar; eauto.
   Qed.
       
-  Definition adaptivePredict (pm  : production_map)
-                             (cm  : closure_map)
-                             (o   : option nonterminal)
-                             (x   : nonterminal)
-                             (suf : list symbol)
-                             (frs : list suffix_frame)
-                             (ts  : list token)
-                             (ca  : cache)
-                             (hc  : cache_stores_target_results pm cm ca)
-                             (hk  : stack_pushes_from_keyset pm (SF o (NT x :: suf), frs)):
-                             prediction_result * cache :=
-    let sll_res := sllPredict pm cm x ts ca hc
+  Definition adaptivePredict
+             (g   : grammar)
+             (hw  : grammar_wf g)
+             (rm  : rhs_map)
+             (cm  : closure_map)
+             (x   : nonterminal)
+             (pre : list symbol)
+             (vs  : symbols_semty pre)
+             (y   : nonterminal)
+             (suf : list symbol)
+             (frs : list parser_frame)
+             (ts  : list token)
+             (ca  : cache)
+             (hc  : cache_stores_target_results rm cm ca)
+             (hk  : stack_lhss_from_keyset rm (Fr x pre vs (NT y :: suf), frs)) :
+    prediction_result * cache :=
+    let sll_res := sllPredict rm cm y ts ca hc
     in  match sll_res with
-        | (PredAmbig _, _) => (llPredict pm o x suf frs ts hk, ca)
+        | (PredAmbig _, _) => (llPredict g hw rm x pre vs y suf frs ts hk, ca)
         | _                => sll_res
         end.
   
   Lemma adaptivePredict_succ_in_rhssFor :
-    forall pm cm o x suf frs ts ca hc hk ys ca',
-      adaptivePredict pm cm o x suf frs ts ca hc hk = (PredSucc ys, ca')
-      -> In ys (rhssFor x pm).
+    forall g hw rm cm x pre vs y suf frs ts ca hc hk ys ca',
+      adaptivePredict g hw rm cm x pre vs y suf frs ts ca hc hk = (PredSucc ys, ca')
+      -> In ys (rhssFor y rm).
   Proof.
-    intros pm cm o x suf frs ts ca hc hk ys ca' ha.
+    intros g hw rm cm x pre vs y suf frs ts ca hc hk ys ca' ha.
     unfold adaptivePredict in ha; dmeqs h; tc; inv ha.
     - eapply sllPredict_succ_in_rhssFor; eauto.
     - eapply llPredict_succ_in_rhssFor; eauto.
   Qed.
   
   Lemma adaptivePredict_succ_in_grammar :
-    forall g pm cm o x suf frs ts ca hc hk ys ca',
-      production_map_correct pm g
-      -> adaptivePredict pm cm o x suf frs ts ca hc hk = (PredSucc ys, ca')
-      -> In (x, ys) g.
+    forall g hw rm cm x pre vs y suf frs ts ca hc hk ys ca',
+      rhs_map_correct rm g
+      -> adaptivePredict g hw rm cm x pre vs y suf frs ts ca hc hk = (PredSucc ys, ca')
+      -> PM.In (y, ys) g.
   Proof.
-    intros g pm cm o x suf frs ts ca hc hk ys ca' hp ha.
+    intros.
     eapply rhssFor_in_iff; eauto.
     eapply adaptivePredict_succ_in_rhssFor; eauto.
   Qed.
 
   Lemma adaptivePredict_ambig_in_grammar :
-    forall g pm cm o x suf frs ts ca hc hk ys ca',
-      production_map_correct pm g
-      -> adaptivePredict pm cm o x suf frs ts ca hc hk = (PredAmbig ys, ca')
-      -> In (x, ys) g.
+    forall g hw rm cm x pre vs y suf frs ts ca hc hk ys ca',
+      rhs_map_correct rm g
+      -> adaptivePredict g hw rm cm x pre vs y suf frs ts ca hc hk = (PredAmbig ys, ca')
+      -> PM.In (y, ys) g.
   Proof.
-    intros g pm cm o x suf frs ts ca hc hk ys ca' hp ha.
+    intros g hw rm cm x pre vs y suf frs ts ca hc hk ys ca' hp ha.
     unfold adaptivePredict in ha; dms; tc; inv ha.
     eapply llPredict_ambig_in_grammar; eauto.
   Qed.
 
   Lemma adaptivePredict_succ_preserves_cache_invar :
-    forall pm cm o x suf frs ts ca hc hk ys ca',
-      adaptivePredict pm cm o x suf frs ts ca hc hk = (PredSucc ys, ca')
-      -> cache_stores_target_results pm cm ca'.
+    forall g hw rm cm x pre vs y suf frs ts ca hc hk ys ca',
+      adaptivePredict g hw rm cm x pre vs y suf frs ts ca hc hk = (PredSucc ys, ca')
+      -> cache_stores_target_results rm cm ca'.
   Proof.
-    intros pm cm o x suf frs ts ca hc hk ys ca' ha.
+    intros g hw rm cm x pre vs y suf frs ts ca hc hk ys ca' ha.
     unfold adaptivePredict in ha; dmeqs H; inv ha; auto.
     eapply sllPredict_succ_preserves_cache_invar; eauto.
   Qed.
 
   Lemma adaptivePredict_ambig_preserves_cache_invar :
-    forall pm cm o x suf frs ts ca hc hk ys ca',
-      adaptivePredict pm cm o x suf frs ts ca hc hk = (PredAmbig ys, ca')
-      -> cache_stores_target_results pm cm ca'.
+    forall g hw rm cm x pre vs y suf frs ts ca hc hk ys ca',
+      adaptivePredict g hw rm cm x pre vs y suf frs ts ca hc hk = (PredAmbig ys, ca')
+      -> cache_stores_target_results rm cm ca'.
   Proof.
-    intros pm cm o x suf frs ts ca hc hk ys ca' ha.
+    intros g hw rm cm x pre vs y suf frs ts ca hc hk ys ca' ha.
     unfold adaptivePredict in ha; dmeqs H; inv ha; auto.
   Qed.
   
 End SllPredictionFn.
+ 
